[wip] various fixes on embedding compcert

compcertox/KRel.v
@@ -18,51 +18,50 @@ Definition blocks (se: Genv.symtbl) (names: ident -> Prop) : block -> Z -> Prop 
 
 (** The relation Rr is parametrized by the symbol table so that we do not have
     to bind the variables being abstracted to particular blocks *)
-Record krel {K1 K2: Type}: Type :=
+Record krel' {K1 K2: Type}: Type :=
   mk_krel {
-      krel_rel (se: Genv.symtbl):> K2 -> mem * K1 -> Prop;
+      krel_pred (se: Genv.symtbl):> K2 -> mem * K1 -> Prop;
       (** the names of the static variables being abstracted *)
-      vars : ident -> Prop;
-      (** other variables *)
-      others := fun i => ~ vars i;
+      krel_footprint : ident -> Prop;
 
       (** the abstraction relation is not affected by other variables *)
-      G_unchanged: forall se k1 k2 m m',
-        krel_rel se k2 (m, k1) -> Mem.unchanged_on (blocks se vars) m m' -> krel_rel se k2 (m', k1);
+      krel_invar: forall se k1 k2 m m',
+        krel_pred se k2 (m, k1) ->
+        Mem.unchanged_on (blocks se krel_footprint) m m' ->
+        krel_pred se k2 (m', k1);
       (** the abstraction relation only focuses on valid blocks, i.e. those have
           been allocated *)
-      G_valid: forall se k1 k2 m b ofs,
-        krel_rel se k2 (m, k1) -> (blocks se vars) b ofs -> Mem.valid_block m b;
+      krel_valid: forall se k1 k2 m b ofs,
+        krel_pred se k2 (m, k1) -> (blocks se krel_footprint) b ofs -> Mem.valid_block m b;
     }.
-Arguments krel: clear implicits.
+Arguments krel': clear implicits.
 
 Section KREL_KCC.
 
-  Context {K1 K2} (R: krel K2 K1).
-  Context (se: Genv.symtbl).
+  Context {K1 K2} (R: krel' K2 K1).
 
-  Inductive krel_kcc_query: query (li_c @ K1) -> query (li_c @ K2) -> Prop :=
+  Inductive krel_kcc_query se: query (li_c @ K1) -> query (li_c @ K2) -> Prop :=
     krel_kcc_query_intro vf1 vf2 sg vargs1 vargs2 m1 m2 k1 k2:
       Val.inject inject_id vf1 vf2 -> Val.inject_list inject_id vargs1 vargs2 ->
-      Mem.extends m1 m2 -> vf1 <> Vundef -> no_perm_on m1 (blocks se (vars R)) ->
-      krel_rel R se k1 (m2, k2) ->
-      krel_kcc_query (cq vf1 sg vargs1 m1, k1) (cq vf2 sg vargs2 m2, k2).
-  Inductive krel_kcc_reply: reply (li_c @ K1) -> reply (li_c @ K2) -> Prop :=
+      Mem.extends m1 m2 -> vf1 <> Vundef -> no_perm_on m1 (blocks se (krel_footprint R)) ->
+      krel_pred R se k1 (m2, k2) ->
+      krel_kcc_query se (cq vf1 sg vargs1 m1, k1) (cq vf2 sg vargs2 m2, k2).
+  Inductive krel_kcc_reply se: reply (li_c @ K1) -> reply (li_c @ K2) -> Prop :=
     krel_kcc_reply_intro vres1 m1 vres2 m2 k1 k2:
       Val.inject inject_id vres1 vres2 ->
-      Mem.extends m1 m2 -> no_perm_on m1 (blocks se (vars R)) ->
-      krel_rel R se k1 (m2, k2) ->
-      krel_kcc_reply (cr vres1 m1, k1) (cr vres2 m2, k2).
+      Mem.extends m1 m2 -> no_perm_on m1 (blocks se (krel_footprint R)) ->
+      krel_pred R se k1 (m2, k2) ->
+      krel_kcc_reply se (cr vres1 m1, k1) (cr vres2 m2, k2).
 
   (* Instance symtbl_kf: KripkeFrame unit Genv.symtbl := *)
   (*   {| acc _ := eq; |}. *)
 
   Program Definition krel_kcc: callconv (li_c @ K1) (li_c @ K2) :=
     {|
-      ccworld := unit;
-      match_senv _ := eq;
-      match_query _ := krel_kcc_query;
-      match_reply _ := krel_kcc_reply;
+      ccworld := Genv.symtbl;
+      match_senv se := fun se1 se2 => se = se1 /\ se = se2;
+      match_query := krel_kcc_query;
+      match_reply := krel_kcc_reply;
     |}.
   Next Obligation.
     inv H0. cbn. apply val_inject_id in H4. inv H4; easy.
@@ -76,36 +75,392 @@ End KREL_KCC.
 Ltac unchanged_implies_solve:=
   eapply Mem.unchanged_on_implies; [eauto | intros b ofs [v [? ?]]; eexists; eauto].
 
+Require Import CallconvAlgebra.
+Require Import Lia.
+
 Section COMP.
 
   (* TODO: Do we need the assumption that R and S do not overlap *)
-  Context {K1 K2 K3} (R: krel K1 K2) (S: krel K2 K3).
+  Context {K1 K2 K3} (R: krel' K1 K2) (S: krel' K2 K3).
 
   Local Obligation Tactic := cbn.
   (* TODO: Promoting to callconv preserves composition *)
-  Program Definition krel_comp: krel K1 K3 :=
+  Program Definition krel_comp: krel' K1 K3 :=
     {|
-      krel_rel se :=
+      krel_pred se :=
         fun k3 '(m1, k1) => exists k2, S se k3 (m1, k2) /\ R se k2 (m1, k1);
-      vars i := vars S i \/ vars R i;
+      krel_footprint i := krel_footprint S i \/ krel_footprint R i;
     |}.
   Next Obligation.
     intros se k1 k3 m1 m1' (k2 & HS & HR) H.
     eexists k2. split.
-    - eapply G_unchanged; eauto.
+    - eapply krel_invar; eauto.
       unchanged_implies_solve.
-    - eapply G_unchanged; eauto.
+    - eapply krel_invar; eauto.
       unchanged_implies_solve.
   Qed.
   Next Obligation.
     intros se k1 k3 * (k2 & HS & HR) Hb.
     unfold blocks in Hb. destruct Hb as (v & Hv & ?).
     destruct Hv.
-    - eapply G_valid. apply HS.
+    - eapply krel_valid. apply HS.
       exists v; split; auto.
-    - eapply G_valid. apply HR.
+    - eapply krel_valid. apply HR.
       exists v; split; auto.
       Unshelve. apply ofs. apply ofs.
   Qed.
 
+  Lemma krel_comp_ref:
+    ccref (krel_kcc S @ krel_kcc R)%cc (krel_kcc krel_comp).
+  Proof.
+    intros [[se wr] ws].
+    intros se1 se2 (q3 & k3) (q1 & k1) Hse Hq. cbn in *.
+    inv Hse. inv H. inv H0.
+    eexists. split. split; reflexivity.
+    split.
+    - destruct Hq as ((q2 & k2) & Hq1 & Hq2).
+      inversion Hq1 as [ ? ? ? ? ? ? ? ? ? Hf1 Hargs1 Hm1 Hvf1 Hperm1 Hr1 ].
+      inversion Hq2 as [ ? ? ? ? ? ? ? ? ? Hf2 Hargs2 Hm2 Hvf2 Hperm2 Hr2 ].
+      subst. clear Hq1 Hq2. inv H3.
+      constructor; eauto.
+      + eapply Mem.val_lessdef_inject_compose. 2: eauto.
+        apply val_inject_id. eauto.
+      + admit.
+      + eapply Mem.extends_extends_compose; eauto.
+      + unfold no_perm_on in *. intros * Hb. cbn in Hb.
+        destruct Hb as [i [[Hi|Hi] Hb]].
+        * apply Hperm1. eexists; split; eauto.
+        * intros contra. eapply Hperm2.
+          eexists; split; eauto. instantiate (1 := ofs).
+          eapply Mem.perm_extends; eauto.
+      + exists k2. split; eauto.
+        eapply krel_invar; eauto.
+        constructor.
+        * erewrite Mem.mext_next. reflexivity. eauto.
+        * intros * Hb Hvb. split.
+          -- apply Mem.perm_extends. eauto.
+          -- intros Hp. eapply Mem.mext_perm_inv in Hp; eauto.
+             destruct Hp; eauto.
+             admit.
+        * intros * Hb Hperm.
+          eapply Mem.mext_inj in Hm2.
+          exploit (Mem.mi_memval _ _ _ Hm2). 2: apply Hperm.
+          unfold inject_id. reflexivity.
+          intros Hv. replace (ofs + 0) with ofs in Hv by lia.
+          inv Hv.
+          -- reflexivity.
+          -- admit.
+          -- admit.
+    - intros [r3 k3'] [r1 k1'] Hr.
+      inversion Hr as [v3 m3 v1 m1 ? ? Hv Hm Hperm Hk]. subst. clear Hr.
+      destruct Hk as [k2' [HS HR]].
+      exists ((cr v1 m1), k2'). split.
+      + constructor; eauto. admit.
+      + constructor; eauto.
+        * reflexivity.
+        * apply Mem.extends_refl.
+        * admit.
+  Abort.
+
 End COMP.
+
+Module KCC.
+
+  Section CKLR.
+
+    Context {K1 K2} (R: @krel' K2 K1).
+
+    Inductive kworld := kw (se: Genv.symtbl) (k1: K1) (k2: K2).
+
+    Inductive krel_mm : kworld -> mem -> mem -> Prop :=
+      match_intro: forall se k1 k2 m1 m2,
+          Mem.extends m1 m2 -> krel_pred R se k1 (m2, k2) ->
+          (* The source program would crash if it tries to manipulate data on blocks
+             defined in the footprint *)
+          no_perm_on m1 (blocks se (krel_footprint R)) ->
+          krel_mm (kw se k1 k2) m1 m2.
+    Inductive krel_match_se: kworld -> Genv.symtbl -> Genv.symtbl -> Prop :=
+      match_se_intro: forall se k1 k2, krel_match_se (kw se k1 k2) se se.
+
+    Program Definition krel_cklr: cklr :=
+      {|
+        world := kworld;
+        wacc := eq;
+        mi w := inject_id;
+        match_mem := krel_mm;
+        match_stbls := krel_match_se;
+      |}.
+    (* mi_acc *)
+    Next Obligation. repeat rstep. apply inject_incr_refl. Qed.
+    (* match_stbls_acc *)
+    Next Obligation. rauto. Qed.
+    (* match_stbls_proj *)
+    Next Obligation.
+      intros se1 se2 Hse. inv Hse. apply Genv.match_stbls_id.
+    Qed.
+    (* match_stbls_nextblock *)
+    Next Obligation.
+      inv H. inv H0. erewrite <- Mem.mext_next; eauto.
+    Qed.
+    (* cklr_alloc *)
+    Next Obligation.
+      intros [ ] m1 m2 Hm lo hi. inv Hm.
+      destruct (Mem.alloc m1 lo hi) as [m1' b1] eqn: Hm1.
+      edestruct Mem.alloc_extends as (m2' & Hm2' & Hm'); eauto; try reflexivity.
+      rewrite Hm2'.
+      eexists; split; repeat rstep.
+      constructor; auto.
+      - eapply krel_invar; eauto.
+        eapply Mem.alloc_unchanged_on; eauto.
+      - unfold no_perm_on in *. intros.
+        specialize (H6 _ _ H). intros Hp. apply H6.
+        eapply Mem.perm_alloc_4 in Hp; eauto.
+        eapply Mem.alloc_result in Hm1. subst.
+        eapply krel_valid in H5; eauto.
+        erewrite Mem.mext_next; eauto.
+    Qed.
+    (* cklr_free *)
+    Next Obligation.
+      intros [ ] m1 m2 Hm [[b lo] hi] r2 Hr. inv Hm.
+      apply coreflexivity in Hr. subst. simpl. red.
+      destruct (Mem.free m1 b lo hi) as [m1'|] eqn:Hm1'; [|constructor].
+      edestruct Mem.free_parallel_extends as (m2' & Hm2' & Hm'); eauto.
+      rewrite Hm2'. constructor.
+      eexists; split; repeat rstep.
+      constructor; auto.
+      - eapply krel_invar; eauto.
+        eapply Mem.free_unchanged_on; eauto.
+        intros ofs Hofs Hv. specialize (H6 _ _ Hv). apply H6.
+        exploit Mem.free_range_perm. apply Hm1'. eauto.
+        intros Hp. eapply Mem.perm_cur_max.
+        eapply Mem.perm_implies. apply Hp. constructor.
+      - unfold no_perm_on in *. intros.
+        specialize (H6 _ _ H). intros Hp. apply H6.
+        eapply Mem.perm_free_3; eauto.
+    Qed.
+    (* cklr_load *)
+    Next Obligation.
+      intros [ ] chunk m1 m2 Hm [b ofs] p2 Hp. inv Hm.
+      apply coreflexivity in Hp; subst. simpl. red.
+      destruct (Mem.load chunk m1 b ofs) as [v1|] eqn:Hv1; [|constructor].
+      edestruct Mem.load_extends as (v2 & Hv2 & Hv); eauto.
+      rewrite Hv2. rewrite val_inject_lessdef_eqrel. rauto.
+    Qed.
+    (* cklr_store *)
+    Next Obligation.
+      intros [ ] chunk m1 m2 Hm [b ofs] p2 Hp v1 v2 Hv. inv Hm.
+      apply coreflexivity in Hp; subst. simpl. red.
+      destruct (Mem.store chunk m1 b ofs v1) as [m1'|] eqn:Hm1'; [|constructor].
+      apply val_inject_lessdef in Hv.
+      edestruct Mem.store_within_extends as (m2' & Hm2' & Hm'); eauto.
+      rewrite Hm2'. constructor.
+      eexists _; split; repeat rstep.
+      constructor; auto.
+      - eapply krel_invar; eauto.
+        eapply Mem.store_unchanged_on; eauto.
+        intros ofs' Hofs. intros Hp. specialize (H6 _ _ Hp). apply H6.
+        exploit Mem.store_valid_access_3. apply Hm1'.
+        unfold Mem.valid_access. intros [Hpr ?]. specialize (Hpr _ Hofs).
+        eapply Mem.perm_cur_max. eapply Mem.perm_implies. apply Hpr. constructor.
+      - unfold no_perm_on in *. intros.
+        specialize (H6 _ _ H). intros Hp. apply H6.
+        eapply Mem.perm_store_2; eauto.
+    Qed.
+    (* cklr_loadbytes *)
+    Next Obligation.
+      intros [ ] m1 m2 Hm [b ofs] p2 Hp sz. inv Hm.
+      apply coreflexivity in Hp; subst. simpl. red.
+      destruct (Mem.loadbytes m1 b ofs sz) as [v1|] eqn:Hv1; [|constructor].
+      edestruct Mem.loadbytes_extends as (v2 & Hv2 & Hv); eauto.
+      rewrite Hv2. rauto.
+    Qed.
+    (* cklr_storebytes *)
+    Next Obligation.
+      intros [ ] m1 m2 Hm [b1 ofs1] p2 Hp vs1 vs2 Hv. inv Hm.
+      apply coreflexivity in Hp. subst. simpl. red.
+      destruct (Mem.storebytes m1 b1 ofs1 vs1) as [m1'|] eqn:Hm1'; [|constructor].
+      edestruct Mem.storebytes_within_extends as (m2' & Hm2' & Hm'); eauto.
+      eapply list_rel_forall2. apply Hv.
+      rewrite Hm2'. constructor.
+      eexists _; split; repeat rstep.
+      constructor; auto.
+      - eapply krel_invar; eauto.
+        eapply Mem.storebytes_unchanged_on; eauto.
+        intros ofs' Hofs. intros Hp. specialize (H6 _ _ Hp). apply H6.
+        exploit Mem.storebytes_range_perm. apply Hm1'.
+        rewrite length_rel; eauto. intros.
+        eapply Mem.perm_cur_max. eapply Mem.perm_implies; eauto. constructor.
+      - unfold no_perm_on in *. intros.
+        specialize (H6 _ _ H). intros Hp. apply H6.
+        eapply Mem.perm_storebytes_2; eauto.
+    Qed.
+    (* cklr_perm *)
+    Next Obligation.
+      intros [ ] m1 m2 Hm [b1 ofs1] p2 Hp p' ? H. inv Hm.
+      apply coreflexivity in Hp. subst. simpl in *.
+      eapply Mem.perm_extends; eauto.
+    Qed.
+    (* cklr_valid_block *)
+    Next Obligation.
+      intros [ ] m1 m2 Hm b1 b2 Hb. inv Hm.
+      apply coreflexivity in Hb. subst.
+      apply Mem.valid_block_extends; eauto.
+    Qed.
+    (* cklr_no_overlap *)
+    Next Obligation.
+      intros b1 b1' delta1 b2 b2' delta2 ofs1 ofs2 Hb Hb1' Hb2' Hp1 Hp2. inv H.
+      inv Hb1'. inv Hb2'. eauto.
+    Qed.
+    (* cklr_representable *)
+    Next Obligation. xomega. Qed.
+    (* cklr_aligned_area_inject *)
+    Next Obligation. rewrite Z.add_0_r. assumption. Qed.
+    (* cklr_disjoint_or_equal_inject *)
+    Next Obligation. intuition xomega. Qed.
+    (* cklr_perm_inv *)
+    Next Obligation.
+      inv H0. unfold inject_id in *. inv H3.
+      replace (ofs1 + 0) with ofs1 in *; try omega.
+      inv H. eapply Mem.perm_extends_inv; eauto.
+    Qed.
+    (* cklr_nextblock_incr *)
+    Next Obligation.
+      destruct H0 as (w' & Hw' & H'). inv Hw'.
+      inv H. inv H'.
+      apply Mem.mext_next in H0.
+      apply Mem.mext_next in H5.
+      rewrite H0. rewrite H5. reflexivity.
+    Qed.
+
+  End CKLR.
+
+End KCC.
+
+Section SIMULATION.
+  Context {K1 K2} (R: @krel' K2 K1).
+
+  Lemma cont_match_mr w w' k1 k2:
+    cont_match (KCC.krel_cklr R) w k1 k2 ->
+    cont_match (KCC.krel_cklr R) w' k1 k2.
+  Proof.
+    induction 1; try constructor; auto.
+  Qed.
+
+  Lemma clight_sim p: forward_simulation (krel_kcc R) (krel_kcc R) (semantics2 p @ K1) (semantics2 p @ K2).
+  Proof.
+    constructor. econstructor; eauto. intros i. reflexivity.
+    instantiate (1 := fun _ _ _ => _). cbn beta.
+    intros ? se w Hse Hse1. inv Hse. cbn -[semantics2] in *.
+    pose (ms := fun '(s1, k1) '(s2, k2) =>
+                  Clightrel.state_match (KCC.krel_cklr R) (KCC.kw se k1 k2) s1 s2).
+    apply forward_simulation_step with (match_states := ms).
+    - intros [q1 k1] [q2 k2] [s1 k1'] Hq Hs1. inv Hq. inv Hs1.
+      cbn in *. subst k1'. inv H. cbn in *.
+      exists (Callstate vf2 vargs2 Kstop m2, k2). split.
+      + constructor; auto. cbn.
+        econstructor; eauto.
+        * unfold globalenv. cbn.
+          exploit (@find_funct_inject p (KCC.krel_cklr R) (KCC.kw se k1 k2) (globalenv se p)).
+          split; cbn; eauto.
+          eapply (rel_push_rintro (fun se => globalenv se p) (fun se => globalenv se p)).
+          constructor. eauto. intro Hx. apply Hx.
+        * eapply val_casted_list_inject; eauto.
+        * simpl. eapply match_stbls_nextblock; eauto.
+          instantiate (2 := KCC.krel_cklr R). instantiate (1 := KCC.kw se k1 k2).
+          constructor. constructor; auto.
+      + constructor; auto. cbn.
+        apply list_inject_subrel'.
+        auto. constructor. constructor; auto.
+    - intros [s1 k1] [s2 k2] [r1 k1'] Hs Hfinal.
+      inv Hfinal. cbn in *. subst k1'. inv H. inv Hs. inv H5.
+      eexists (_, k2). split. split; cbn; auto.
+      + inv H4. econstructor.
+      + constructor; cbn; auto.
+    - intros [s1 k1] [s2 k2] [q1 k1'] Hs Hext.
+      inv Hext. cbn in *. subst k1'. inv H. inv Hs. inv H8.
+      eexists se, (_, _). repeat apply conj; cbn; eauto.
+      + cbn. econstructor.
+        exploit (@find_funct_inject p (KCC.krel_cklr R) (KCC.kw se k1 k2) (globalenv se p)).
+        split; cbn; eauto.
+        eapply (rel_push_rintro (fun se => globalenv se p) (fun se => globalenv se p)).
+        constructor. eauto. intros Hx. subst f. apply Hx.
+      + constructor; cbn; auto.
+        eapply list_inject_subrel. auto.
+        destruct vf; cbn in *; congruence.
+      + intros [r1 kr1] [r2 kr2] [s1' k1'] Hr [Hafter H].
+        inv Hafter. cbn in *. subst k1'. inv Hr. inv H.
+        cbn in *. eexists (_, kr2). split. split; auto.
+        cbn. econstructor.
+        constructor; auto. eapply cont_match_mr. eauto.
+        constructor; auto.
+    - intros [s1 k1] t [s1' k1'] Hstep [s2 k2] Hs.
+      inv Hstep. cbn in H.
+      exploit step2_rel; eauto. unfold genv_match.
+      eapply (rel_push_rintro (fun se => globalenv se p) (fun se => globalenv se p)).
+      constructor. intros (s2' & Hstep' & w' & Hw' & Hs').
+      exists (s2', k2). inv Hw'. split; auto.
+      constructor. apply Hstep'. reflexivity.
+    - apply well_founded_ltof.
+  Qed.
+
+End SIMULATION.
+
+Unset Asymmetric Patterns.
+
+Inductive krel: Type -> Type -> Type :=
+| krel_singleton {K1 K2} : krel' K1 K2 -> krel K1 K2
+| krel_compose {K1 K2 K3} : krel K1 K2 -> krel K2 K3 -> krel K1 K3.
+
+Fixpoint krel_cc {K1 K2} (rel: krel K1 K2): callconv (li_c @ K2) (li_c @ K1) :=
+  match rel with
+  | krel_singleton r => krel_kcc r
+  | krel_compose r1 r2 => (krel_cc r2) @ (krel_cc r1)
+  end.
+
+Coercion krel_cc : krel >-> callconv.
+
+Lemma clight_krel {K1 K2} (R: krel K2 K1) p:
+  forward_simulation R R (Clight.semantics2 p @ K1) (Clight.semantics2 p @ K2).
+Proof.
+  induction R; simpl.
+  - apply clight_sim.
+  - eapply compose_forward_simulations; eauto.
+Qed.
+
+Require Import SmallstepLinking.
+Require Import compcertox.CModule.
+
+Lemma cmodule_krel {K1 K2} (R: @krel K2 K1) M sk:
+  skel_module_compatible M sk ->
+  forward_simulation R R (semantics M sk @ K1) (semantics M sk @ K2).
+Proof.
+  intros Hsk.
+
+  eapply open_fsim_ccref. apply cc_compose_id_left.
+  unfold flip. apply cc_compose_id_left.
+  eapply compose_forward_simulations.
+  apply lift_horizontal_comp1.
+
+  eapply open_fsim_ccref. apply cc_compose_id_right.
+  unfold flip. apply cc_compose_id_right.
+  eapply compose_forward_simulations.
+  2: { apply lift_horizontal_comp2. }
+
+  apply semantics_simulation'.
+  - intros. induction M as [| p ps]; try easy.
+    destruct i.
+    + cbn. apply clight_krel.
+    + apply IHps.
+      unfold skel_module_compatible in *.
+      rewrite -> Forall_forall in *.
+      intros x Hx. apply Hsk. right. auto.
+  - intros. induction M as [| p ps]; try easy.
+    destruct i.
+    + cbn. unfold skel_module_compatible in *.
+      rewrite -> Forall_forall in *. apply Hsk.
+      left. auto.
+    + apply IHps.
+      unfold skel_module_compatible in *.
+      rewrite -> Forall_forall in *.
+      intros x Hx. apply Hsk. right. auto.
+Qed.
